WIP: max_top wbisim max_op

dataplane/Examples/Max_top.thy
@@ -30,9 +30,9 @@ lemma step_max'_top_elim:
   obtains
   x where  "io = Inp None (Inl (Inl x))" "op = \<oslash>"
 | x where  "io = Inp None (Inr x)" "op = \<oslash>"
-| st impf ft where "io = Inp None (Inl (Inr impf))" "ft = frontier (impf (0 :: 1))"
+| impf ft where "io = Inp None (Inl (Inr impf))" "ft = frontier (impf (0 :: 1))"
   "is_empty_antichain ft" "op = \<oslash>"
-| st impf ft below result where "io = Inp None (Inl (Inr impf))" "ft = frontier (impf (0 :: 1))"
+| impf ft below result where "io = Inp None (Inl (Inr impf))" "ft = frontier (impf (0 :: 1))"
   "\<not> is_empty_antichain ft" "below = [(n, c) \<leftarrow> buf. less_than_frontier ft (time c)]" "result = maxs below"
   "op = push (Write (max_top' [(n, c) \<leftarrow> buf. \<not> less_than_frontier ft (time c)]) None (Inl (Inl \<lparr> cons = [], inte = map (\<lambda> c. (out c, time c, -1)) (map snd below), prod = map (\<lambda> c. (out c, time c, 1)) (map snd result)\<rparr>)) ) 0 result"
 | x t n where "io = Inp (Some 0) (Inr (n, t))"
@@ -94,9 +94,142 @@ abbreviation "inp_m_top i inps buf1 buf2 \<equiv> map_op (case_sum id id) (case_
 
 
 
-lemma wbcr_trans:
-  "\<W> R x y \<Longrightarrow> \<W> R y z \<Longrightarrow> \<W> R x z"
-  sorry
+lemma wbcr_aux:
+  "bisim_cong R x y \<Longrightarrow> \<W> R x z"
+  oops
+
+find_theorems "\<W>"
+
+term bisim_cong
+
+inductive wbisim_cong_alt for R where
+  wbc_base[intro]:  "R x y \<Longrightarrow> wbisim_cong_alt R x y"
+| wbc_bisim:  "wbisim x y \<Longrightarrow> wbisim_cong_alt R x y"
+| wbc_refl[intro]: "x = y \<Longrightarrow> wbisim_cong_alt R x y"
+| wbc_sym[intro]: "wbisim_cong_alt R x y \<Longrightarrow> wbisim_cong_alt R y x"
+| wbc_Read:"x1 = y1 \<Longrightarrow> rel_fun (=) (wbisim_cong_alt R) x2 y2 \<Longrightarrow> wbisim_cong_alt R (Read x1 x2) (Read y1 y2)"
+| wbc_Write: "wbisim_cong_alt R x1 y1 \<Longrightarrow> wbisim_cong_alt R (Write x1 x2 x3) (Write y1 x2 x3)"
+| wbc_Silent: "wbisim_cong_alt R x1 y1 \<Longrightarrow> wbisim_cong_alt R (Silent x1) (Silent y1)"
+| wbc_bisim_cong: "bisim_cong R x y \<Longrightarrow> wbisim_cong_alt R x y"
+
+lemma wbisim_cong_alt_disj:
+  "(wbisim_cong_alt R x y \<or> wbisim x y) = wbisim_cong_alt R x y"
+  by (auto intro: wbc_bisim)
+
+
+lemma wbisim_coinduct_upto[consumes 1, case_names BISIM]:
+  "R op1 op2 \<Longrightarrow>
+   (\<And>s t. R s t \<Longrightarrow> wsim (wbisim_cong_alt R) s t \<and> wsim (wbisim_cong_alt R) t s) \<Longrightarrow>
+   op1 \<approx> op2"
+  apply (rule wbisim.coinduct[where X="wbisim_cong_alt R", unfolded wbisim_cong_alt_disj, of op1 op2])
+  subgoal
+    by (auto intro: wbc_bisim)
+  subgoal premises prems for s' t'
+    using prems(3) apply -
+    apply (induct s' t' rule: wbisim_cong_alt.induct)
+    subgoal for op1 op2
+      by (drule prems(2)) auto
+    subgoal for op1 op2
+      using wsim_mono[of wbisim "wbisim_cong_alt R"]
+      apply (auto simp: le_fun_def wbc_bisim elim: wbisim.cases)
+      done
+    subgoal for op1 op2
+      by (auto simp: wsim_def wstep_def)
+    subgoal for op1 op2
+      by fastforce
+    subgoal for p q f g
+      by (auto simp: rel_fun_def intro!: step_wstep[OF SR])
+    subgoal for op1 op2 p x
+      by (auto intro!: step_wstep[OF SW])
+    subgoal for op1 op2
+      by (auto intro: wsim_SilentI)
+    subgoal for op1 op2
+      oops
+
+inductive converges where
+  ceq[intro]: "op1 = op2 \<Longrightarrow> converges op1 op2"
+| cstep: "(\<And>io. step io op1 op1' \<Longrightarrow> step io op2 op2' \<Longrightarrow> converges op1' op2') \<Longrightarrow> converges op1 op2"
+
+
+lemma
+  "converges 
+   (dataflow_op sg
+     (map_op (case_sum id id) (case_sum id id)
+       (comp_op [Inr (0 :: 2, 1 :: 1) \<mapsto> Inr (1 :: 2, 1)] (BENQ (Inr (1, 1)) (Inr (n, i)) buf1)
+         (map_op (case_option (Inl 0) (\<lambda>p. Inr (0, 1))) (case_option (Inl 0) (\<lambda>p. Inr (0, 1)))
+           (writes (Write (input_top (Cap (Suc i) 1) inps1') None (Inl (Inl \<lparr>cons = [], inte = [(1, i, - 1), (1, Suc i, 1)], prod = [(1, i, 1 + int (length xs))]\<rparr>))) (Some 1) (map (\<lambda>x. Inr (x, i)) xs)))
+         (map_op (case_option (Inl 1) (\<lambda>p. Inr (1, 1))) (case_option (Inl 1) (\<lambda>p. Inr (1, 1))) (max_top' buf2)))))
+    (dataflow_op (sg\<lparr>lo_pt := lo_pt sg @ extract_progress 0 (\<lambda>l. if node l = 0 \<and> port l = Src 1 then [Loc 1 (Trg 0)] else []) \<lparr>cons = [], inte = [], prod = [(1, i, 1)]\<rparr>\<rparr>)
+     (map_op (case_sum id id) (case_sum id id)
+       (comp_op [Inr (0, 1) \<mapsto> Inr (1, 1)] (BENQ (Inr (1, 1)) (Inr (n, i)) buf1) (map_op (case_option (Inl 0) (\<lambda>p. Inr (0, 1))) (case_option (Inl 0) (\<lambda>p. Inr (0, 1))) (input_top (Cap i 1) (LCons xs inps1')))
+         (map_op (case_option (Inl 1) (\<lambda>p. Inr (1, 1))) (case_option (Inl 1) (\<lambda>p. Inr (1, 1))) (max_top' buf2)))))"
+  apply (cases xs)
+  subgoal
+    apply simp
+  apply (rule cstep)
+  subgoal for io
+    apply (cases io)
+    defer
+    subgoal for p x
+      apply (cases p; simp)
+      apply (erule step_dataflow_op_elim)
+      apply (elim step_map_op_elim conjE step_comp_op_elim; simp; hypsubst_thin)
+      subgoal for a nid pa op1' xa
+        apply hypsubst_thin
+        oops
+
+lemma aux2:
+  "step io op1 (Write opf (Inl nid) (Inl (Inl st))) \<Longrightarrow>
+   step io op2 (Write opf (Inl nid) (Inl (Inl \<lparr>cons = [], inte = [], prod = []\<rparr>))) \<Longrightarrow>
+   dataflow_op sg op1 = dataflow_op (sg\<lparr> lo_pt := lo_pt sg @ extract_progress nid (edges sg) st \<rparr>) op2"
+  apply (coinduction arbitrary: op1 op2 rule: op.coinduct_upto)
+  apply simp
+  subgoal for op1 op2
+    apply (subst (3 4) dataflow_op.code)
+    apply (simp add: rel_set_image split: sum.splits option.splits op.splits)
+    apply (rule rel_setI)
+    subgoal for op
+(*       apply (auto 0 0 simp add: rel_set_image split: sum.splits option.splits op.splits)
+      subgoal for f p opp
+        apply hypsubst_thin *)
+        oops
+
+(* FIXME: move me *)
+lemma steps_writes:
+  "ios = map (Out p) xs \<Longrightarrow>
+   steps ios (writes op p xs) op"
+  apply (induct ios arbitrary: xs)
+   apply (force simp add: writes_Cons_simp)+
+  done
+
+lemma
+  "dataflow_op sg
+     (map_op (case_sum id id) (case_sum id id)
+       (comp_op [Inr (0, 1) \<mapsto> Inr (1, 1)] buf
+         (map_op (case_option (Inl 0) (\<lambda>p. Inr (0, 1))) (case_option (Inl 0) (\<lambda>p. Inr (0, 1)))
+           (writes (Write op1 None (Inl (Inl \<lparr>cons = cs, inte = is, prod = ps\<rparr>))) (Some 1) (map (\<lambda>x. Inr (x, i)) xs)))
+         (map_op (case_option (Inl 1) (\<lambda>p. Inr (1, 1))) (case_option (Inl 1) (\<lambda>p. Inr (1, 1))) op2))) =
+    dataflow_op (sg\<lparr>lo_pt := lo_pt sg @ extract_progress 0 (\<lambda>l. if node l = 0 \<and> port l = Src 1 then [Loc 1 (Trg 0)] else []) \<lparr>cons = cs, inte = is, prod = ps\<rparr>\<rparr>)
+     (map_op (case_sum id id) (case_sum id id)
+       (comp_op [Inr (0, 1) \<mapsto> Inr (1, 1)] buf
+         (map_op (case_option (Inl 0) (\<lambda>p. Inr (0, 1))) (case_option (Inl 0) (\<lambda>p. Inr (0, 1)))
+           (writes
+             (Write op1 None
+               (Inl (Inl \<lparr>cons = [], inte = [], prod = []\<rparr>)))
+             (Some 1) (map ((\<lambda>(x, c). Inr (x, time c)) \<circ> (\<lambda>x. (x, Cap i 1))) xs)))
+         (map_op (case_option (Inl 1) (\<lambda>p. Inr (1, 1))) (case_option (Inl 1) (\<lambda>p. Inr (1, 1))) op2)))"
+  apply (induct xs arbitrary: ps "is" cs)
+  subgoal 
+    apply simp
+    apply (subst (1 2) dataflow_op.code)
+    apply (auto 0 0 simp del: cfilter_eq simp add: extract_progress_def split: op.splits if_splits option.splits)
+    subgoal for p f
+      apply (cases p; auto split: option.splits)
+      subgoal for p x
+        apply (rule cimage_eqI[simplified, of _ _ "Read (Inl p) f"])
+         apply simp_all
+        subgoal
+          oops
 
 lemma
   \<open>ys @@- xs @@- lconcat (lmap (\<lambda> (xs, t). map (\<lambda> n. (n, t)) xs) (lzip inps1 (iterates Suc i))) =
@@ -122,7 +255,6 @@ proof (coinduction arbitrary: inps1 inps2 buf1 buf2 inrbufs1 xs ys i j sg rule: 
           apply (rule exI)
           apply (rule conjI)
            apply (rule rtranclp.intros(1))
-          apply (rule wbcr_trans[rotated])
           apply (rule wbcr_base)
           apply (rule exI[of _ "LCons xs' inps1'"])
           apply (rule exI[of _ "inps2"])
@@ -132,21 +264,92 @@ proof (coinduction arbitrary: inps1 inps2 buf1 buf2 inrbufs1 xs ys i j sg rule: 
           apply (rule exI[of _ "j"])
           apply (rule exI[of _ "sg\<lparr> lo_pt := (lo_pt sg) @ extract_progress 0 (edges sg) \<lparr>cons = [], inte = [], prod = [(1, i, 1)]\<rparr> \<rparr>"])
           apply simp
-          apply (intro conjI)
-            apply (rule refl)
+          apply (intro conjI[rotated])
           subgoal
             apply (drule sym)
             apply simp
             subgoal premises prems
               apply (rule arg_cong2[where f=lshift])
                apply simp_all
-          apply (rule arg_cong2[where f=lshift])
+              apply (rule arg_cong2[where f=lshift])
                apply (simp_all add: lconcat_correct)
               apply (subst (1 2) iterates.code)
               apply simp
               done
             done
-          subgoal
+          subgoal premises
+            apply (cases xs')
+            subgoal
+              apply simp
+            apply (coinduction rule: op.coinduct_upto)
+            apply simp
+            apply (rule rel_setI)
+            subgoal for op
+              apply (auto 0 0 split: op.splits)
+              subgoal for p f
+                apply (cases p; simp split: option.splits sum.splits)
+                subgoal for p' pttr
+                  apply hypsubst_thin
+                  apply (rule bexI[of _ "Read (Inl p') f"])
+                   apply simp
+                  subgoal
+                    apply auto
+        apply (rule op.cong_Silent)
+                    apply (rule op.cong_base)
+                    apply auto
+                    subgoal for pttr'
+                      apply (drule Read_in_choices_step[simplified, where x="Inl (Inr (\<lambda>p. c_imp pttr (Loc p' (Trg 1))))"])
+                      apply (elim exE step_map_op_elim step_comp_op_elim conjE step_max'_top_elim; simp; hypsubst_thin)
+                      subgoal for x io' op'' p 
+                        by auto
+                      subgoal for x io' op'' p op2' io'a op''a
+                        apply (drule sym[of _ "f (Inl (Inr (\<lambda>p. c_imp pttr (Loc 1 (Trg 1)))))"])
+                        apply simp
+                        apply (subst (2) comp_op_code)
+                        apply simp
+
+end
+                        apply (cases x; simp)
+                        subgoal for a
+                        apply (cases a; simp)
+                          subgoal
+                            apply hypsubst_thin
+                            apply (subgoal_tac "c_imp pttr (Loc 1 (Trg 1)) = c_imp pttr' (Loc 1 (Trg 1))")
+                            subgoal
+                            apply auto
+
+                            apply (cases io; simp split: option.splits)
+
+                      find_theorems choices step
+
+
+end
+    done
+  subgoal for a xs' 
+    apply (subst (1 2) writes.code)
+    apply simp
+    apply (subst (1 2) dataflow_op.code)
+    apply (simp add: extract_progress_def split: option.splits sum.splits)
+    done
+  done
+
+end
+              apply (subst ( ) aux)
+              apply (simp add: extract_progress_def)
+              apply (rule dataflow_op_change_multiplicities)
+              apply simp_all
+
+end
+              apply (smt (verit, del_insts) Cons_eq_appendI append.left_neutral change_multiplicities_append change_multiplicities_comm)
+              done
+            subgoal
+              apply (subst (1 2) aux)
+              
+
+              find_theorems dataflow_op change_multiplicities
+
+
+
           apply (rule wbcr_bisim)
 
           done
